(Not completely finished) proofs that int31 integers fulfill the CyclicAxioms specs
Currently, 8 lemmas remains to tackle. One proof is done via a _very_
brute-force ugly approach. The all story for proving composition of
phi and phi_inv (and the other way around) is surprisingly long and
tricky. In both cases, comments are welcome, I may have missed an
easier road (?)

As a consequence of the above, we have a additional time-eager
file in the stdlib (about a minute to compile here). 



git-svn-id: svn+ssh://scm.gforge.inria.fr/svn/coq/trunk@10973 85f007b7-540e-0410-9357-904b9bb8a0f7

theories/Numbers/Cyclic/Int31/Cyclic31.v
@@ -11,100 +11,1617 @@
 (** * Int31 numbers defines indeed a cyclic structure : Z/(2^31)Z *)
 
 (**
-Author: Arnaud Spiwack
+Author: Arnaud Spiwack (+ Pierre Letouzey)
 *)
 
 Require Export Int31.
+Require Import Znumtheory.
 Require Import CyclicAxioms.
+Require Import ROmega.
 
+Open Scope nat_scope.
 Open Scope int31_scope.
 
-Definition int31_op : znz_op int31.
- split.
+Section Basics.
 
- (* Conversion functions with Z *)
- exact (31%positive). (* number of digits *)
- exact (31). (* number of digits *)
- exact (phi). (* conversion to Z *)
- exact (positive_to_int31). (* positive -> N*int31 :  p => N,i where p = N*2^31+phi i *)
- exact head031.  (* number of head 0 *)
- exact tail031.  (* number of tail 0 *)
+ (** Auxiliary lemmas. To migrate later *)
 
- (* Basic constructors *)
- exact 0. (* 0 *)
- exact 1. (* 1 *)
- exact Tn. (* 2^31 - 1 *)
- (* A function which given two int31 i and j, returns a double word
+ Lemma Zdouble_spec : forall z, Zdouble z = (2*z)%Z.
+ Proof.
+ reflexivity.
+ Qed.
+
+ Lemma Zdouble_plus_one_spec : forall z, Zdouble_plus_one z = (2*z+1)%Z.
+ Proof.
+ destruct z; simpl; auto with zarith.
+ Qed.
+
+
+ (** * Basic results about [iszero], [shiftl], [shiftr] *)
+
+ Lemma iszero_eq0 : forall x, iszero x = true -> x=0.
+ Proof.
+ destruct x; simpl; intros.
+ repeat 
+   match goal with H:(if ?d then _ else _) = true |- _ => 
+     destruct d; try discriminate 
+   end.
+ reflexivity.
+ Qed.
+
+ Lemma iszero_not_eq0 : forall x, iszero x = false -> x<>0.
+ Proof.
+ intros x H Eq; rewrite Eq in H; simpl in *; discriminate.
+ Qed.
+
+ Lemma sneakl_shiftr : forall x, 
+  x = sneakl (firstr x) (shiftr x).
+ Proof.
+ destruct x; simpl; auto.
+ Qed.
+
+ Lemma sneakr_shiftl : forall x, 
+  x = sneakr (firstl x) (shiftl x).
+ Proof.
+ destruct x; simpl; auto.
+ Qed.
+
+ Lemma twice_zero : forall x, 
+  twice x = 0 <-> twice_plus_one x = 1.
+ Proof.
+ destruct x; simpl in *; split; 
+ intro H; injection H; intros; subst; auto.
+ Qed.
+
+ Lemma twice_or_twice_plus_one : forall x, 
+  x = twice (shiftr x) \/ x = twice_plus_one (shiftr x).
+ Proof.
+ intros; case_eq (firstr x); intros.
+ destruct x; simpl in *; rewrite H; auto.
+ destruct x; simpl in *; rewrite H; auto.
+ Qed.
+
+
+
+ (** * Iterated shift to the right *)
+
+ Definition nshiftr n x := iter_nat n _ shiftr x.
+
+ Lemma nshiftr_S : 
+  forall n x, nshiftr (S n) x = shiftr (nshiftr n x).
+ Proof.
+ reflexivity.
+ Qed.
+
+ Lemma nshiftr_S_tail : 
+  forall n x, nshiftr (S n) x = nshiftr n (shiftr x).
+ Proof.
+ induction n; simpl; auto.
+ intros; rewrite nshiftr_S, IHn, nshiftr_S; auto.
+ Qed.
+
+ Lemma nshiftr_n_0 : forall n, nshiftr n 0 = 0.
+ Proof.
+ induction n; simpl; auto.
+ rewrite nshiftr_S, IHn; auto.
+ Qed.
+
+ Lemma nshiftr_size : forall x, nshiftr size x = 0.
+ Proof.
+ destruct x; simpl; auto.
+ Qed.
+
+ Lemma nshiftr_above_size : forall k x, size<=k -> 
+  nshiftr k x = 0.
+ Proof.
+ intros.
+ replace k with ((k-size)+size)%nat by omega.
+ induction (k-size)%nat; auto.
+  rewrite nshiftr_size; auto.
+  simpl; rewrite nshiftr_S, IHn; auto.
+ Qed.
+
+ (** * Iterated shift to the left *)
+
+ Definition nshiftl n x := iter_nat n _ shiftl x.
+
+ Lemma nshiftl_S : 
+  forall n x, nshiftl (S n) x = shiftl (nshiftl n x).
+ Proof.
+ reflexivity.
+ Qed.
+
+ Lemma nshiftl_S_tail : 
+  forall n x, nshiftl (S n) x = nshiftl n (shiftl x).
+ Proof.
+ induction n; simpl; auto.
+ intros; rewrite nshiftl_S, IHn, nshiftl_S; auto.
+ Qed.
+
+ Lemma nshiftl_n_0 : forall n, nshiftl n 0 = 0.
+ Proof.
+ induction n; simpl; auto.
+ rewrite nshiftl_S, IHn; auto.
+ Qed.
+
+ Lemma nshiftl_size : forall x, nshiftl size x = 0.
+ Proof.
+ destruct x; simpl; auto.
+ Qed.
+
+ Lemma nshiftl_above_size : forall k x, size<=k -> 
+  nshiftl k x = 0.
+ Proof.
+ intros.
+ replace k with ((k-size)+size)%nat by omega.
+ induction (k-size)%nat; auto.
+  rewrite nshiftl_size; auto.
+  simpl; rewrite nshiftl_S, IHn; auto.
+ Qed.
+
+ Lemma firstr_firstl : 
+  forall x, firstr x = firstl (nshiftl (pred size) x).
+ Proof.
+ destruct x; simpl; auto.
+ Qed.
+ 
+ (** More advanced results about [nshiftr] *)
+
+ Lemma nshiftr_predsize_0_firstl : forall x, 
+  nshiftr (pred size) x = 0 -> firstl x = D0.
+ Proof.
+ destruct x; compute; intros H; injection H; intros; subst; auto.
+ Qed.
+
+ Lemma nshiftr_0_propagates : forall n p x, n <= p -> 
+  nshiftr n x = 0 -> nshiftr p x = 0.
+ Proof.
+ intros.
+ replace p with ((p-n)+n)%nat by omega.
+ induction (p-n)%nat.
+ simpl; auto.
+ simpl; rewrite nshiftr_S; rewrite IHn0; auto.
+ Qed.
+
+ Lemma nshiftr_0_firstl : forall n x, n < size -> 
+  nshiftr n x = 0 -> firstl x = D0.
+ Proof.
+ intros.
+ apply nshiftr_predsize_0_firstl.
+ apply nshiftr_0_propagates with n; auto; omega.
+ Qed.
+
+ (** * Some induction principles over [int31] *)
+
+ (** Not used for the moment. Are they really useful ? *)
+
+ Lemma int31_ind_sneakl : forall P : int31->Prop,
+  P 0 -> 
+  (forall x d, P x -> P (sneakl d x)) ->  
+  forall x, P x.
+ Proof.
+ intros.
+ assert (forall n, n<=size -> P (nshiftr (size - n) x)).
+ induction n; intros.
+ rewrite nshiftr_size; auto.
+ rewrite sneakl_shiftr.
+ apply H0.
+ change (P (nshiftr (S (size - S n)) x)).
+ replace (S (size - S n))%nat with (size - n)%nat by omega.
+ apply IHn; omega.
+ change x with (nshiftr (size-size) x); auto.
+ Qed.
+
+ Lemma int31_ind_twice : forall P : int31->Prop, 
+  P 0 -> 
+  (forall x, P x -> P (twice x)) ->  
+  (forall x, P x -> P (twice_plus_one x)) ->  
+  forall x, P x.
+ Proof.
+ induction x using int31_ind_sneakl; auto.
+ destruct d; auto.
+ Qed.
+
+
+ (** * Some generic results about [recr] *)
+
+ Section Recr.
+ 
+ (** [recr] satisfies the fixpoint equation used for its definition. *)
+
+ Variable (A:Type)(case0:A)(caserec:digits->int31->A->A).
+ 
+ Lemma recr_aux_eqn : forall n x, iszero x = false -> 
+   recr_aux (S n) A case0 caserec x = 
+   caserec (firstr x) (shiftr x) (recr_aux n A case0 caserec (shiftr x)).
+ Proof.
+ intros; simpl; rewrite H; auto.
+ Qed.
+
+ Lemma recr_aux_converges : 
+  forall n p x, n <= size -> n <= p ->
+  recr_aux n A case0 caserec (nshiftr (size - n) x) = 
+  recr_aux p A case0 caserec (nshiftr (size - n) x).
+ Proof.
+ induction n.
+ simpl; intros.
+ rewrite nshiftr_size; destruct p; simpl; auto.
+ intros.
+ destruct p.
+ inversion H0.
+ unfold recr_aux; fold recr_aux.
+ destruct (iszero (nshiftr (size - S n) x)); auto.
+ f_equal.
+ change (shiftr (nshiftr (size - S n) x)) with (nshiftr (S (size - S n)) x).
+ replace (S (size - S n))%nat with (size - n)%nat by omega.
+ apply IHn; auto with arith.
+ Qed.
+
+ Lemma recr_eqn : forall x, iszero x = false -> 
+  recr A case0 caserec x = 
+  caserec (firstr x) (shiftr x) (recr A case0 caserec (shiftr x)).
+ Proof.
+ intros.
+ unfold recr.
+ change x with (nshiftr (size - size) x).
+ rewrite (recr_aux_converges size (S size)); auto with arith.
+ rewrite recr_aux_eqn; auto.
+ Qed.
+ 
+ (** [recr] is usually equivalent to a variant [recrbis] 
+     written without [iszero] check. *)
+
+ Fixpoint recrbis_aux (n:nat)(A:Type)(case0:A)(caserec:digits->int31->A->A) 
+ (i:int31) : A :=
+  match n with
+  | O => case0
+  | S next =>
+      let si := shiftr i in
+      caserec (firstr i) si (recrbis_aux next A case0 caserec si)
+  end.
+ 
+ Definition recrbis := recrbis_aux size.
+
+ Hypothesis case0_caserec : caserec D0 0 case0 = case0.
+
+ Lemma recrbis_aux_equiv : forall n x,
+   recrbis_aux n A case0 caserec x = recr_aux n A case0 caserec x.
+ Proof.
+ induction n; simpl; auto; intros.
+ case_eq (iszero x); intros; [ | f_equal; auto ].
+ rewrite (iszero_eq0 _ H); simpl; auto.
+ replace (recrbis_aux n A case0 caserec 0) with case0; auto.
+ clear H IHn; induction n; simpl; congruence.
+ Qed.
+ 
+ Lemma recrbis_equiv : forall x, 
+   recrbis A case0 caserec x = recr A case0 caserec x.
+ Proof.
+ intros; apply recrbis_aux_equiv; auto.
+ Qed.
+
+ End Recr.
+
+ (** * Incrementation *)
+
+ Section Incr.
+
+ (** Variant of [incr] via [recrbis] *)
+
+ Let Incr (b : digits) (si rec : int31) :=
+  match b with
+   | D0 => sneakl D1 si
+   | D1 => sneakl D0 rec
+  end.
+
+ Definition incrbis_aux n x := recrbis_aux n _ In Incr x.
+
+ Lemma incrbis_aux_equiv : forall x, incrbis_aux size x = incr x.
+ Proof.
+ unfold incr, recr, incrbis_aux; fold Incr; intros.
+ apply recrbis_aux_equiv; auto.
+ Qed.
+
+ (** Recursive equations satisfied by [incr] *)
+
+ Lemma incr_eqn1 :
+  forall x, firstr x = D0 -> incr x = twice_plus_one (shiftr x).
+ Proof.
+ intros.
+ case_eq (iszero x); intros.
+ rewrite (iszero_eq0 _ H0); simpl; auto.
+ unfold incr; rewrite recr_eqn; fold incr; auto.
+ rewrite H; auto.
+ Qed.
+
+ Lemma incr_eqn2 :
+  forall x, firstr x = D1 -> incr x = twice (incr (shiftr x)).
+ Proof.
+ intros.
+ case_eq (iszero x); intros.
+ rewrite (iszero_eq0 _ H0) in H; simpl in H; discriminate.
+ unfold incr; rewrite recr_eqn; fold incr; auto.
+ rewrite H; auto.
+ Qed.
+
+ Lemma incr_twice : forall x, incr (twice x) = twice_plus_one x.
+ Proof.
+ intros.
+ rewrite incr_eqn1; destruct x; simpl; auto.
+ Qed.
+
+ Lemma incr_twice_plus_one_firstl : 
+  forall x, firstl x = D0 -> incr (twice_plus_one x) = twice (incr x).
+ Proof.
+ intros.
+ rewrite incr_eqn2; [ | destruct x; simpl; auto ].
+ f_equal; f_equal.
+ destruct x; simpl in *; rewrite H; auto.
+ Qed.
+ 
+ (** The previous result is actually true even without the 
+     constraint on [firstl], but this is harder to prove 
+     (see later). *)
+
+ End Incr.
+
+ (** * Conversion to [Z] : the [phi] function *)
+
+ Section Phi.
+
+ (** Variant of [phi] via [recrbis] *)
+
+ Let Phi := fun b (_:int31) => 
+       match b with D0 => Zdouble | D1 => Zdouble_plus_one end.
+ 
+ Definition phibis_aux n x := recrbis_aux n _ Z0 Phi x.
+
+ Lemma phibis_aux_equiv : forall x, phibis_aux size x = phi x.
+ Proof.
+ unfold phi, recr, phibis_aux; fold Phi; intros.
+ apply recrbis_aux_equiv; auto.
+ Qed.
+
+ (** Recursive equations satisfied by [phi] *)
+
+ Lemma phi_eqn1 : forall x, firstr x = D0 -> 
+  phi x = Zdouble (phi (shiftr x)).
+ Proof.
+ intros.
+ case_eq (iszero x); intros.
+ rewrite (iszero_eq0 _ H0); simpl; auto.
+ intros; unfold phi; rewrite recr_eqn; fold phi; auto.
+ rewrite H; auto.
+ Qed.
+
+ Lemma phi_eqn2 : forall x, firstr x = D1 -> 
+  phi x = Zdouble_plus_one (phi (shiftr x)).
+ Proof.
+ intros.
+ case_eq (iszero x); intros.
+ rewrite (iszero_eq0 _ H0) in H; simpl in H; discriminate.
+ intros; unfold phi; rewrite recr_eqn; fold phi; auto.
+ rewrite H; auto.
+ Qed.
+
+ Lemma phi_twice_firstl : forall x, firstl x = D0 -> 
+  phi (twice x) = Zdouble (phi x).
+ Proof.
+ intros.
+ rewrite phi_eqn1; auto; [ | destruct x; auto ].
+ f_equal; f_equal.
+ destruct x; simpl in *; rewrite H; auto.
+ Qed.
+
+ Lemma phi_twice_plus_one_firstl : forall x, firstl x = D0 -> 
+  phi (twice_plus_one x) = Zdouble_plus_one (phi x).
+ Proof.
+ intros.
+ rewrite phi_eqn2; auto; [ | destruct x; auto ].
+ f_equal; f_equal.
+ destruct x; simpl in *; rewrite H; auto.
+ Qed.
+
+ End Phi.
+
+ (** [phi x] is positive and lower than [2^31] *)
+
+ Lemma phibis_aux_bounded : 
+  forall n x, n <= size -> 
+  (0 <= phibis_aux n (nshiftr (size-n) x) < 2 ^ (Z_of_nat n))%Z.
+ Proof.
+ induction n.
+ simpl; unfold phibis_aux; simpl; auto with zarith.
+ intros.
+ unfold phibis_aux, recrbis_aux; fold recrbis_aux; 
+  fold (phibis_aux n (shiftr (nshiftr (size - S n) x))).
+ assert (shiftr (nshiftr (size - S n) x) =  nshiftr (size-n) x).
+  replace (size - n)%nat with (S (size - (S n))) by omega.
+  simpl; auto.
+ rewrite H0.
+ destruct (IHn x).
+ omega.
+ set (y:=phibis_aux n (nshiftr (size - n) x)) in *.
+ rewrite inj_S, Zpow_facts.Zpower_Zsucc; auto with zarith.
+ case_eq (firstr (nshiftr (size - S n) x)); intros.
+ rewrite Zdouble_spec; auto with zarith.
+ rewrite Zdouble_plus_one_spec; auto with zarith.
+ Qed.
+
+ Lemma phi_bounded  : forall x, (0 <= phi x < 2 ^ (Z_of_nat size))%Z.
+ Proof.
+ intros.
+ rewrite <- phibis_aux_equiv.
+ change x with (nshiftr (size-size) x).
+ apply phibis_aux_bounded; auto.
+ Qed.
+
+ (** * Equivalence modulo [2^n] *)
+
+ Section EqShiftL.
+
+ (** after killing [n] bits at the left, are the numbers equal ?*) 
+
+ Definition EqShiftL n x y :=  
+  nshiftl n x = nshiftl n y.
+
+ Lemma EqShiftL_zero : forall x y, EqShiftL O x y <-> x = y.
+ Proof.
+ unfold EqShiftL; intros; unfold nshiftl; simpl; split; auto.
+ Qed.
+
+ Lemma EqShiftL_size : forall k x y, size<=k -> EqShiftL k x y.
+ Proof.
+ red; intros; rewrite 2 nshiftl_above_size; auto.
+ Qed.
+
+ Lemma EqShiftL_le : forall k k' x y, k <= k' -> 
+   EqShiftL k x y -> EqShiftL k' x y.
+ Proof.
+ unfold EqShiftL; intros.
+ replace k' with ((k'-k)+k)%nat by omega.
+ remember (k'-k)%nat as n.
+ clear Heqn H k'.
+ induction n; simpl; auto.
+ rewrite 2 nshiftl_S; f_equal; auto.
+ Qed.
+
+ Lemma EqShiftL_firstr : forall k x y, k < size -> 
+  EqShiftL k x y -> firstr x = firstr y.
+ Proof.
+ intros.
+ rewrite 2 firstr_firstl.
+ f_equal.
+ apply EqShiftL_le with k; auto. 
+ unfold size.
+ auto with arith.
+ Qed.
+
+ Lemma EqShiftL_twice : forall k x y, 
+  EqShiftL k (twice x) (twice y) <-> EqShiftL (S k) x y.
+ Proof.
+ intros; unfold EqShiftL.
+ rewrite 2 nshiftl_S_tail; split; auto.
+ Qed.
+
+ Lemma twice_equal_equiv : forall x y,
+  twice x = twice y <-> twice_plus_one x = twice_plus_one y.
+ Proof. 
+ destruct x; destruct y; split; intro H; injection H; intros; subst; auto.
+ Qed.
+
+ (** Ugly brute-force proof. Don't know yet how to do otherwise. *)
+
+ Lemma EqShiftL_twice_plus_one : forall k x y, 
+  EqShiftL k (twice_plus_one x) (twice_plus_one y) <-> EqShiftL (S k) x y.
+ Proof.
+ intros; unfold EqShiftL.
+ destruct x; destruct y.
+ do 31
+   (destruct k;
+    [split; intro H; try injection H; intros; subst; auto| ]).
+ split; intros; apply EqShiftL_size; auto with arith.
+ unfold size; omega.
+ unfold size; omega.
+ Qed.
+
+ Lemma EqShiftL_shiftr : forall k x y, EqShiftL k x y -> 
+  EqShiftL (S k) (shiftr x) (shiftr y).
+ Proof.
+ intros.
+ destruct (le_lt_dec size (S k)).
+ apply EqShiftL_size; auto.
+ case_eq (firstr x); intros.
+ rewrite <- EqShiftL_twice.
+ unfold twice; rewrite <- H0.
+ rewrite <- sneakl_shiftr.
+ rewrite (EqShiftL_firstr k x y); auto.
+ rewrite <- sneakl_shiftr; auto.
+ omega.
+ rewrite <- EqShiftL_twice_plus_one.
+ unfold twice_plus_one; rewrite <- H0.
+ rewrite <- sneakl_shiftr.
+ rewrite (EqShiftL_firstr k x y); auto.
+ rewrite <- sneakl_shiftr; auto.
+ omega.
+ Qed.
+
+ Lemma EqShiftL_incrbis : forall n k x y, n<=size -> 
+  (n+k=S size)%nat ->
+  EqShiftL k x y -> 
+  EqShiftL k (incrbis_aux n x) (incrbis_aux n y).
+ Proof.
+ induction n; simpl; intros.
+ red; auto.
+ destruct (eq_nat_dec k size). 
+  subst k; apply EqShiftL_size; auto.
+ unfold incrbis_aux; simpl; 
+  fold (incrbis_aux n (shiftr x)); fold (incrbis_aux n (shiftr y)).
+
+ rewrite (EqShiftL_firstr k x y); auto; try omega.
+ case_eq (firstr y); intros.
+ rewrite EqShiftL_twice_plus_one.
+ apply EqShiftL_shiftr; auto.
+ 
+ rewrite EqShiftL_twice.
+ apply IHn; try omega.
+ apply EqShiftL_shiftr; auto.
+ Qed.
+
+ Lemma EqShiftL_incr : forall x y, 
+  EqShiftL 1 x y -> EqShiftL 1 (incr x) (incr y).
+ Proof.
+ intros.
+ rewrite <- 2 incrbis_aux_equiv.
+ apply EqShiftL_incrbis; auto.
+ Qed.
+ 
+ End EqShiftL.
+
+ (** * More equations about [incr] *)
+
+(*
+ Lemma incr_twice : forall x, incr (twice x) = twice_plus_one x.
+ Proof.
+ intros.
+ rewrite incr_eqn1; destruct x; simpl; auto.
+ Qed.
+*)
+ Lemma incr_twice_plus_one : 
+  forall x, incr (twice_plus_one x) = twice (incr x).
+ Proof.
+ intros.
+ rewrite incr_eqn2; [ | destruct x; simpl; auto].
+ apply EqShiftL_incr.
+ red; destruct x; simpl; auto.
+ Qed.
+
+ Lemma incr_firstr : forall x, firstr (incr x) <> firstr x.
+ Proof.
+ intros.
+ case_eq (firstr x); intros.
+ rewrite incr_eqn1; auto.
+ destruct (shiftr x); simpl; discriminate.
+ rewrite incr_eqn2; auto.
+ destruct (incr (shiftr x)); simpl; discriminate.
+ Qed.
+
+ Lemma incr_inv : forall x y, 
+  incr x = twice_plus_one y -> x = twice y.
+ Proof.
+ intros.
+ case_eq (iszero x); intros.
+ rewrite (iszero_eq0 _ H0) in *; simpl in *.
+ change (incr 0) with 1 in H.
+ symmetry; rewrite twice_zero; auto.
+ case_eq (firstr x); intros.
+ rewrite incr_eqn1 in H; auto.
+ clear H0; destruct x; destruct y; simpl in *.
+ injection H; intros; subst; auto.
+ elim (incr_firstr x).
+ rewrite H1, H; destruct y; simpl; auto.
+ Qed.
+
+ (** * More equations about [phi] *)
+
+ (** * Conversion from [Z] : the [phi_inv] function *)
+
+ (** First, recursive equations *)
+
+ Lemma phi_inv_double_plus_one : forall z, 
+   phi_inv (Zdouble_plus_one z) = twice_plus_one (phi_inv z).
+ Proof.
+ destruct z; simpl; auto.
+ induction p; simpl.
+ rewrite 2 incr_twice; auto.
+ rewrite incr_twice, incr_twice_plus_one.
+ f_equal.
+ apply incr_inv; auto.
+ auto.
+ Qed.
+
+ Lemma phi_inv_double : forall z, 
+   phi_inv (Zdouble z) = twice (phi_inv z).
+ Proof.
+ destruct z; simpl; auto.
+ rewrite incr_twice_plus_one; auto.
+ Qed.
+
+ Lemma phi_inv_incr : forall z, 
+  phi_inv (Zsucc z) = incr (phi_inv z).
+ Proof.
+ destruct z.
+ simpl; auto.
+ simpl; auto.
+ induction p; simpl; auto.
+ rewrite Pplus_one_succ_r, IHp, incr_twice_plus_one; auto.
+ rewrite incr_twice; auto.
+ simpl; auto.
+ destruct p; simpl; auto.
+ rewrite incr_twice; auto.
+ f_equal.
+ rewrite incr_twice_plus_one; auto.
+ induction p; simpl; auto.
+ rewrite incr_twice; auto.
+ f_equal.
+ rewrite incr_twice_plus_one; auto.
+ Qed.
+
+ (** [phi_inv o inv], the always-exact and easy-to-prove trip : 
+     from int31 to Z and then back to int31. *)
+
+ Lemma phi_inv_phi_aux : 
+  forall n x, n <= size -> 
+   phi_inv (phibis_aux n (nshiftr (size-n) x)) = 
+   nshiftr (size-n) x.
+ Proof.
+ induction n.
+ intros; simpl.
+ rewrite nshiftr_size; auto.
+ intros.
+ unfold phibis_aux, recrbis_aux; fold recrbis_aux; 
+  fold (phibis_aux n (shiftr (nshiftr (size-S n) x))).
+ assert (shiftr (nshiftr (size - S n) x) = nshiftr (size-n) x).
+  replace (size - n)%nat with (S (size - (S n))); auto; omega.
+ rewrite H0.
+ case_eq (firstr (nshiftr (size - S n) x)); intros.
+
+ rewrite phi_inv_double.
+ rewrite IHn by omega.
+ rewrite <- H0.
+ remember (nshiftr (size - S n) x) as y.
+ destruct y; simpl in H1; rewrite H1; auto.
+
+ rewrite phi_inv_double_plus_one.
+ rewrite IHn by omega.
+ rewrite <- H0.
+ remember (nshiftr (size - S n) x) as y.
+ destruct y; simpl in H1; rewrite H1; auto.
+ Qed.
+
+ Lemma phi_inv_phi : forall x, phi_inv (phi x) = x.
+ Proof.
+ intros.
+ rewrite <- phibis_aux_equiv.
+ replace x with (nshiftr (size - size) x) by auto.
+ apply phi_inv_phi_aux; auto.
+ Qed.
+
+ (** * [positive_to_int31] *)
+
+ (** A variant of [p2i] with [twice] and [twice_plus_one] instead of 
+     [2*i] and [2*i+1] *)
+
+ Fixpoint p2ibis n p : (N*int31)%type := 
+  match n with
+    | O => (Npos p, On)
+    | S n => match p with
+               | xO p => let (r,i) := p2ibis n p in (r, twice i)
+               | xI p => let (r,i) := p2ibis n p in (r, twice_plus_one i)
+               | xH => (N0, In)
+             end
+  end.
+
+ Lemma p2ibis_bounded : forall n p,  
+  nshiftr n (snd (p2ibis n p)) = 0.
+ Proof.
+ induction n.
+ simpl; intros; auto.
+ simpl; intros.
+ destruct p; simpl.
+
+ specialize IHn with p.
+ destruct (p2ibis n p); simpl in *.
+ rewrite nshiftr_S_tail.
+ destruct (le_lt_dec size n).
+ rewrite nshiftr_above_size; auto.
+ assert (H:=nshiftr_0_firstl _ _ l IHn).
+ replace (shiftr (twice_plus_one i)) with i; auto.
+ destruct i; simpl in *; rewrite H; auto.
+
+ specialize IHn with p.
+ destruct (p2ibis n p); simpl in *.
+ rewrite nshiftr_S_tail.
+ destruct (le_lt_dec size n).
+ rewrite nshiftr_above_size; auto.
+ assert (H:=nshiftr_0_firstl _ _ l IHn).
+ replace (shiftr (twice i)) with i; auto.
+ destruct i; simpl in *; rewrite H; auto.
+
+ rewrite nshiftr_S_tail; auto.
+ replace (shiftr In) with 0; auto.
+ apply nshiftr_n_0.
+ Qed.
+ 
+ Lemma p2ibis_spec : forall n p, n<=size ->
+    Zpos p = ((Z_of_N (fst (p2ibis n p)))*2^(Z_of_nat n) + 
+             phi (snd (p2ibis n p)))%Z.
+ Proof.
+ induction n; intros.
+ simpl; rewrite Pmult_1_r; auto.
+ replace (2^(Z_of_nat (S n)))%Z with (2*2^(Z_of_nat n))%Z by 
+  (rewrite <- Zpow_facts.Zpower_Zsucc, <- Zpos_P_of_succ_nat; 
+   auto with zarith).
+ rewrite (Zmult_comm 2).
+ assert (n<=size) by omega.
+ destruct p; simpl; [ | | auto]; 
+  specialize (IHn p H0); 
+  generalize (p2ibis_bounded n p);
+  destruct (p2ibis n p) as (r,i); simpl in *; intros.
+
+ change (Zpos p~1) with (2*Zpos p + 1)%Z.
+ rewrite phi_twice_plus_one_firstl, Zdouble_plus_one_spec.
+ rewrite IHn; ring.
+ apply (nshiftr_0_firstl n); auto; try omega.
+
+ change (Zpos p~0) with (2*Zpos p)%Z.
+ rewrite phi_twice_firstl.
+ change (Zdouble (phi i)) with (2*(phi i))%Z.
+ rewrite IHn; ring.
+ apply (nshiftr_0_firstl n); auto; try omega.
+ Qed.
+
+ (** We now prove that this [p2ibis] is related to [phi_inv_positive] *)
+
+ Lemma phi_inv_positive_p2ibis : forall n p, (n<=size)%nat -> 
+  EqShiftL (size-n) (phi_inv_positive p) (snd (p2ibis n p)).
+ Proof.
+ induction n.
+ intros.
+ apply EqShiftL_size; auto.
+ intros.
+ simpl p2ibis; destruct p; [ | | red; auto]; 
+  specialize IHn with p; 
+  destruct (p2ibis n p); simpl snd in *; simpl phi_inv_positive; 
+  rewrite ?EqShiftL_twice_plus_one, ?EqShiftL_twice; 
+  replace (S (size - S n))%nat with (size - n)%nat by omega; 
+  apply IHn; omega.
+ Qed.
+
+ (** This gives the expected result about [phi o phi_inv], at least
+     for the positive case. *)
+
+ Lemma phi_phi_inv_positive : forall p, 
+  phi (phi_inv_positive p) = (Zpos p) mod (2^(Z_of_nat size)).
+ Proof.
+ intros.
+ replace (phi_inv_positive p) with (snd (p2ibis size p)).
+ rewrite (p2ibis_spec size p) by auto.
+ rewrite Zplus_comm, Z_mod_plus.
+ symmetry; apply Zmod_small.
+ apply phi_bounded.
+ auto with zarith.
+ symmetry.
+ rewrite <- EqShiftL_zero.
+ apply (phi_inv_positive_p2ibis size p); auto.
+ Qed.
+
+ (** Moreover, [p2ibis] is also related with [p2i] and hence with
+    [positive_to_int31]. *)
+
+ Lemma double_twice_firstl : forall x, firstl x = D0 -> Twon*x = twice x.
+ Proof.
+ intros. 
+ unfold mul31.
+ rewrite <- Zdouble_spec, <- phi_twice_firstl, phi_inv_phi; auto.
+ Qed.
+
+ Lemma double_twice_plus_one_firstl : forall x, firstl x = D0 -> 
+  Twon*x+In = twice_plus_one x.
+ Proof.
+ intros.
+ rewrite double_twice_firstl; auto.
+ unfold add31.
+ rewrite phi_twice_firstl, <- Zdouble_plus_one_spec,
+   <- phi_twice_plus_one_firstl, phi_inv_phi; auto.
+ Qed.
+ 
+ Lemma p2i_p2ibis : forall n p, (n<=size)%nat -> 
+  p2i n p = p2ibis n p.
+ Proof.
+ induction n; simpl; auto; intros.
+ destruct p; auto; specialize IHn with p; 
+  generalize (p2ibis_bounded n p); 
+  rewrite IHn; try omega; destruct (p2ibis n p); simpl; intros; 
+  f_equal; auto.
+ apply double_twice_plus_one_firstl.
+ apply (nshiftr_0_firstl n); auto; omega.
+ apply double_twice_firstl.
+ apply (nshiftr_0_firstl n); auto; omega.
+ Qed.
+
+ Lemma positive_to_int31_phi_inv_positive : forall p, 
+   snd (positive_to_int31 p) = phi_inv_positive p.
+ Proof.
+ intros; unfold positive_to_int31.
+ rewrite p2i_p2ibis; auto.
+ symmetry.
+ rewrite <- EqShiftL_zero.
+ apply (phi_inv_positive_p2ibis size); auto.
+ Qed.
+
+ Lemma positive_to_int31_spec : forall p, 
+    Zpos p = ((Z_of_N (fst (positive_to_int31 p)))*2^(Z_of_nat size) + 
+               phi (snd (positive_to_int31 p)))%Z.
+ Proof.
+ unfold positive_to_int31.
+ intros; rewrite p2i_p2ibis; auto.
+ apply p2ibis_spec; auto.
+ Qed.
+
+ (** Thanks to the result about [phi o phi_inv_positive], we can 
+     now establish easily the most general results about 
+     [phi o twice] and so one. *)
+ 
+ Lemma phi_twice : forall x, 
+   phi (twice x) = (Zdouble (phi x)) mod 2^(Z_of_nat size).
+ Proof.
+ intros.
+ pattern x at 1; rewrite <- (phi_inv_phi x).
+ rewrite <- phi_inv_double.
+ assert (0 <= Zdouble (phi x))%Z.
+  rewrite Zdouble_spec; generalize (phi_bounded x); omega.
+ destruct (Zdouble (phi x)).
+ simpl; auto.
+ apply phi_phi_inv_positive.
+ compute in H; elim H; auto.
+ Qed.
+
+ Lemma phi_twice_plus_one : forall x, 
+   phi (twice_plus_one x) = (Zdouble_plus_one (phi x)) mod 2^(Z_of_nat size).
+ Proof.
+ intros.
+ pattern x at 1; rewrite <- (phi_inv_phi x).
+ rewrite <- phi_inv_double_plus_one.
+ assert (0 <= Zdouble_plus_one (phi x))%Z.
+  rewrite Zdouble_plus_one_spec; generalize (phi_bounded x); omega.
+ destruct (Zdouble_plus_one (phi x)).
+ simpl; auto.
+ apply phi_phi_inv_positive.
+ compute in H; elim H; auto.
+ Qed.
+
+ Lemma phi_incr : forall x, 
+   phi (incr x) = (Zsucc (phi x)) mod 2^(Z_of_nat size).
+ Proof.
+ intros.
+ pattern x at 1; rewrite <- (phi_inv_phi x).
+ rewrite <- phi_inv_incr.
+ assert (0 <= Zsucc (phi x))%Z.
+  change (Zsucc (phi x)) with ((phi x)+1)%Z; 
+   generalize (phi_bounded x); omega.
+ destruct (Zsucc (phi x)).
+ simpl; auto.
+ apply phi_phi_inv_positive.
+ compute in H; elim H; auto.
+ Qed.
+
+ (** With the previous results, we can deal with [phi o phi_inv] even 
+    in the negative case *)
+
+ Lemma phi_phi_inv_negative : 
+  forall p, phi (incr (complement_negative p)) = (Zneg p) mod 2^(Z_of_nat size).
+ Proof.
+ induction p.
+
+ simpl complement_negative.
+ rewrite phi_incr in IHp.
+ rewrite incr_twice, phi_twice_plus_one.
+ remember (phi (complement_negative p)) as q.
+ rewrite Zdouble_plus_one_spec.
+ replace (2*q+1)%Z with (2*(Zsucc q)-1)%Z by omega.
+ rewrite <- Zminus_mod_idemp_l, <- Zmult_mod_idemp_r, IHp.
+ rewrite Zmult_mod_idemp_r, Zminus_mod_idemp_l; auto with zarith.
+
+ simpl complement_negative.
+ rewrite incr_twice_plus_one, phi_twice.
+ remember (phi (incr (complement_negative p))) as q.
+ rewrite Zdouble_spec, IHp, Zmult_mod_idemp_r; auto with zarith.
+ 
+ simpl; auto.
+ Qed.
+
+ Lemma phi_phi_inv : 
+  forall z, phi (phi_inv z) = z mod 2 ^ (Z_of_nat size).
+ Proof.
+ destruct z.
+ simpl; auto.
+ apply phi_phi_inv_positive.
+ apply phi_phi_inv_negative.
+ Qed.
+
+
+End Basics.
+
+
+Section Int31_Op.
+
+(** A function which given two int31 i and j, returns a double word
     which is worth i*2^31+j *)
- exact (fun i j => match (match i ?= 0 with | Eq =>  j ?= 0 | not0 => not0 end) with | Eq => W0 | _ => WW i j end).
- (* two special cases where i and j are respectively taken equal to 0 *)
- exact (fun i => match i ?= 0 with | Eq => W0 | _ => WW i 0 end).
- exact (fun j => match j ?= 0 with | Eq => W0 | _ => WW 0 j end).
+Let w_WW i j := 
+  match (match i ?= 0 with Eq => j ?= 0 | not0 => not0 end) with 
+    | Eq => W0 
+    | _ => WW i j 
+  end.
 
+(** Two special cases where i and j are respectively taken equal to 0 *)
+Let w_W0 i := match i ?= 0 with Eq => W0 | _ => WW i 0 end.
+Let w_0W j := match j ?= 0 with Eq => W0 | _ => WW 0 j end.
+
+(** Nullity test *)
+Let w_iszero i := match i ?= 0 with Eq => true | _ => false end.
+
+(** Modulo [2^p] *)
+Let w_pos_mod p i :=
+  match compare31 p 32 with
+    | Lt => addmuldiv31 p 0 (addmuldiv31 (31-p) i 0)
+    | _ => i
+  end.
+
+(** Parity test *)
+Let w_iseven i := 
+ let (_,r) := i/2 in
+ match r ?= 0 with Eq => true | _ => false end.
+
+Definition int31_op := (mk_znz_op
+ 31%positive (* number of digits *)
+ 31 (* number of digits *)
+ phi (* conversion to Z *)
+ positive_to_int31 (* positive -> N*int31 :  p => N,i where p = N*2^31+phi i *)
+ head031  (* number of head 0 *)
+ tail031  (* number of tail 0 *)
+ (* Basic constructors *)
+ 0
+ 1
+ Tn (* 2^31 - 1 *)
+ w_WW
+ w_W0
+ w_0W
  (* Comparison *)
- exact compare31.
- exact (fun i => match i ?= 0 with | Eq => true | _ => false end).
-
+ compare31
+ w_iszero
  (* Basic arithmetic operations *)
- (* opposite functions *)
- exact (fun i => 0 -c i).
- exact (fun i => 0 - i).
- exact (fun i => 0-i-1). (* the carry is always -1*)
- (* successor and addition functions *)
- exact (fun i => i +c 1).
- exact add31c.
- exact add31carryc.
- exact (fun i => i + 1).
- exact add31.
- exact (fun i j => i + j + 1).
- (* predecessor and subtraction functions *)
- exact (fun i => i -c 1).
- exact sub31c.
- exact sub31carryc.
- exact (fun i => i - 1).
- exact sub31.
- exact (fun i j => i - j - 1).
- (* multiplication functions *)
- exact mul31c.
- exact mul31.
- exact (fun x => x *c x).
-
+ (fun i => 0 -c i)
+ (fun i => 0 - i)
+ (fun i => 0-i-1)
+ (fun i => i +c 1)
+ add31c
+ add31carryc
+ (fun i => i + 1)
+ add31
+ (fun i j => i + j + 1)
+ (fun i => i -c 1)
+ sub31c
+ sub31carryc
+ (fun i => i - 1)
+ sub31
+ (fun i j => i - j - 1)
+ mul31c
+ mul31
+ (fun x => x *c x)
  (* special (euclidian) division operations *)
- exact div3121.
- exact div31. (* this is supposed to be the special case of division a/b where a > b *)
- exact div31.
+ div3121
+ div31 (* this is supposed to be the special case of division a/b where a > b *)
+ div31
  (* euclidian division remainder *)
  (* again special case for a > b *)
- exact (fun i j => let (_,r) := i/j in r).
- exact (fun i j => let (_,r) := i/j in r).
- (* gcd functions *)
- exact gcd31. (*gcd_gt*)
- exact gcd31. (*gcd*)
- 
+ (fun i j => let (_,r) := i/j in r)
+ (fun i j => let (_,r) := i/j in r)
+ gcd31 (*gcd_gt*)
+ gcd31 (*gcd*)
  (* shift operations *)
- exact addmuldiv31. (*add_mul_div  *)
-(*modulo 2^p  *)
- exact (fun p i => 
-     match compare31 p 32 with
-     | Lt => addmuldiv31 p 0 (addmuldiv31 (31-p) i 0)
-     | _ => i
-     end).
-
+ addmuldiv31 (*add_mul_div  *)
+ (* modulo 2^p *)
+ w_pos_mod
  (* is i even ? *)
- exact (fun i => let (_,r) := i/2 in 
-                          match r ?= 0 with
-                          | Eq => true
-                          | _ => false
-                          end).
-
+ w_iseven
  (* square root operations *)
- exact sqrt312. (* sqrt2 *)
- exact sqrt31. (* sqr *)
-Defined.
+ sqrt312 (* sqrt2 *)
+ sqrt31 (* sqrt *)
+).
 
+End Int31_Op.
 
-Definition int31_spec : znz_spec int31_op.
-Admitted.
+Section Int31_Spec.
+ 
+ Open Local Scope Z_scope.
+
+ Notation "[| x |]" := (phi x)  (at level 0, x at level 99).
+
+ Notation Local wB := (2 ^ (Z_of_nat size)).
+ 
+ Lemma wB_pos : wB > 0. 
+ Proof.
+  auto with zarith.
+ Qed.
+
+ Notation "[+| c |]" :=
+   (interp_carry 1 wB phi c)  (at level 0, x at level 99).
+
+ Notation "[-| c |]" :=
+   (interp_carry (-1) wB phi c)  (at level 0, x at level 99).
+
+ Notation "[|| x ||]" :=
+   (zn2z_to_Z wB phi x)  (at level 0, x at level 99).
+
+ Definition spec_to_Z := phi_bounded.
+
+ Lemma spec_zdigits : [| 31%int31 |] = 31.
+ Proof.
+  reflexivity.
+ Qed.
+
+ Lemma spec_more_than_1_digit: 1 < 31.
+ Proof.
+  auto with zarith.
+ Qed.
+
+ Lemma spec_0   : [|0%int31|] = 0.
+ Proof.
+  reflexivity.
+ Qed.
+ 
+ Lemma spec_1   : [|1%int31|] = 1.
+ Proof.
+  reflexivity.
+ Qed.
+    
+ Lemma spec_Bm1 : [|Tn|] = wB - 1.
+ Proof.
+  reflexivity.
+ Qed.
+
+ Lemma spec_compare : forall x y,
+   match compare31 x y with
+     | Eq => [|x|] = [|y|]
+     | Lt => [|x|] < [|y|]
+     | Gt => [|x|] > [|y|]
+   end.
+ Proof.
+ clear; unfold compare31; simpl; intros.
+ case_eq ([|x|] ?= [|y|]); auto.
+ intros; apply Zcompare_Eq_eq; auto.
+ Qed.
+
+ Let w_eq0         := int31_op.(znz_eq0).
+
+ Lemma spec_eq0 : forall x, w_eq0 x = true -> [|x|] = 0.
+ Proof.
+ clear; unfold w_eq0, znz_eq0; simpl.
+ unfold compare31; simpl; intros.
+ change [|0|] with 0 in H.
+ apply Zcompare_Eq_eq.
+ now destruct ([|x|] ?= 0).
+ Qed.
+
+ Let wWW           := int31_op.(znz_WW).
+ Let w0W           := int31_op.(znz_0W).
+ Let wW0           := int31_op.(znz_W0).
+
+ Lemma spec_WW  : forall h l, [||wWW h l||] = [|h|] * wB + [|l|].
+ Proof.
+ clear; unfold wWW; simpl; intros.
+ unfold compare31 in *.
+ change [|0|] with 0.
+ case_eq ([|h|] ?= 0); simpl; auto.
+ case_eq ([|l|] ?= 0); simpl; auto.
+ intros.
+ rewrite (Zcompare_Eq_eq _ _ H); simpl.
+ rewrite (Zcompare_Eq_eq _ _ H0); simpl; auto.
+ Qed.
+
+ Lemma spec_0W  : forall l, [||w0W l||] = [|l|].
+ Proof.
+ clear; unfold w0W; simpl; intros.
+ unfold compare31 in *.
+ change [|0|] with 0.
+ case_eq ([|l|] ?= 0); simpl; auto.
+ intros; symmetry; apply Zcompare_Eq_eq; auto.
+ Qed.
+
+ Lemma spec_W0  : forall h, [||wW0 h||] = [|h|]*wB.
+ Proof.
+ clear; unfold wW0; simpl; intros.
+ unfold compare31 in *.
+ change [|0|] with 0.
+ case_eq ([|h|] ?= 0); simpl; auto with zarith.
+ intro H; rewrite (Zcompare_Eq_eq _ _ H); auto.
+ Qed.
+
+ (** Addition *)
+
+ Let w_add_c       := int31_op.(znz_add_c).
+ Let w_add_carry_c := int31_op.(znz_add_carry_c).
+ Let w_add         := int31_op.(znz_add).
+ Let w_add_carry   := int31_op.(znz_add_carry).
+ Let w_succ        := int31_op.(znz_succ).
+ Let w_succ_c      := int31_op.(znz_succ_c).
+
+ Lemma spec_add_c  : forall x y, [+|w_add_c x y|] = [|x|] + [|y|].
+ Proof.
+ clear; unfold w_add_c, znz_add_c; simpl; intros.
+ unfold add31c, add31, interp_carry; rewrite phi_phi_inv.
+ generalize (spec_to_Z x)(spec_to_Z y); intros.
+ set (X:=[|x|]) in *; set (Y:=[|y|]) in *; clearbody X Y.
+
+ assert ((X+Y) mod wB ?= X+Y <> Eq -> [+|C1 (phi_inv (X+Y))|] = X+Y).
+  unfold interp_carry; rewrite phi_phi_inv, Zcompare_Eq_iff_eq; intros.
+  destruct (Z_lt_le_dec (X+Y) wB).
+  contradict H1; auto using Zmod_small with zarith.
+  rewrite <- (Z_mod_plus_full (X+Y) (-1) wB).
+  rewrite Zmod_small; romega. (* omega : BUG !! (peut-etre a cause du clear) *)
+
+ generalize (Zcompare_Eq_eq ((X+Y) mod wB) (X+Y)); intros Heq.
+ destruct Zcompare; intros; 
+  [ rewrite phi_phi_inv; auto | now apply H1 | now apply H1].
+ Qed.
+
+ Lemma spec_succ_c : forall x, [+|w_succ_c x|] = [|x|] + 1.
+ Proof.
+ clear - w_add_c; unfold w_succ_c, znz_succ_c; simpl; intros.
+ apply spec_add_c. (* erreur gore si clear trop violent *)
+ Qed.
+
+ Lemma spec_add_carry_c : forall x y, [+|w_add_carry_c x y|] = [|x|] + [|y|] + 1.
+ Proof.
+ clear; unfold w_add_carry_c, znz_add_carry_c, int31_op; intros.
+ unfold add31carryc, interp_carry; rewrite phi_phi_inv.
+ generalize (spec_to_Z x)(spec_to_Z y); intros.
+ set (X:=[|x|]) in *; set (Y:=[|y|]) in *; clearbody X Y.
+
+ assert ((X+Y+1) mod wB ?= X+Y+1 <> Eq -> [+|C1 (phi_inv (X+Y+1))|] = X+Y+1).
+  unfold interp_carry; rewrite phi_phi_inv, Zcompare_Eq_iff_eq; intros.
+  destruct (Z_lt_le_dec (X+Y+1) wB).
+  contradict H1; auto using Zmod_small with zarith.
+  rewrite <- (Z_mod_plus_full (X+Y+1) (-1) wB).
+  rewrite Zmod_small; romega.
+
+ generalize (Zcompare_Eq_eq ((X+Y+1) mod wB) (X+Y+1)); intros Heq.
+ destruct Zcompare; intros; 
+  [ rewrite phi_phi_inv; auto | now apply H1 | now apply H1].
+ Qed.
+
+ Lemma spec_add : forall x y, [|w_add x y|] = ([|x|] + [|y|]) mod wB.
+ Proof.
+ clear; unfold w_add; simpl; intros.
+ apply phi_phi_inv.
+ Qed.
+
+ Lemma spec_add_carry :
+	 forall x y, [|w_add_carry x y|] = ([|x|] + [|y|] + 1) mod wB.
+ Proof.
+ clear; unfold w_add_carry, znz_add_carry, int31_op, add31; intros.
+ repeat rewrite phi_phi_inv.
+ apply Zplus_mod_idemp_l.
+ Qed.
+
+ Lemma spec_succ : forall x, [|w_succ x|] = ([|x|] + 1) mod wB.
+ Proof.
+ clear - w_add; unfold w_succ, znz_succ, int31_op; intros.
+ change 1 with [|1|].
+ apply spec_add.
+ Qed.
+
+ (** Substraction *)
+
+ Let w_sub_c       := int31_op.(znz_sub_c).
+ Let w_sub_carry_c := int31_op.(znz_sub_carry_c).
+ Let w_sub         := int31_op.(znz_sub).
+ Let w_sub_carry   := int31_op.(znz_sub_carry).
+ Let w_pred_c      := int31_op.(znz_pred_c).
+ Let w_pred        := int31_op.(znz_pred).
+ Let w_opp_c       := int31_op.(znz_opp_c).
+ Let w_opp         := int31_op.(znz_opp).
+ Let w_opp_carry   := int31_op.(znz_opp_carry).
+
+ Lemma spec_sub_c : forall x y, [-|w_sub_c x y|] = [|x|] - [|y|].
+ Proof. 
+ clear; unfold w_sub_c; simpl; intros.
+ unfold sub31c, sub31, interp_carry; intros.
+ rewrite phi_phi_inv.
+ generalize (spec_to_Z x)(spec_to_Z y); intros.
+ set (X:=[|x|]) in *; set (Y:=[|y|]) in *; clearbody X Y.
+
+ assert ((X-Y) mod wB ?= X-Y <> Eq -> [-|C1 (phi_inv (X-Y))|] = X-Y).
+  unfold interp_carry; rewrite phi_phi_inv, Zcompare_Eq_iff_eq; intros.
+  destruct (Z_lt_le_dec (X-Y) 0).
+  rewrite <- (Z_mod_plus_full (X-Y) 1 wB).
+  rewrite Zmod_small; romega.
+  contradict H1; apply Zmod_small; romega.
+
+ generalize (Zcompare_Eq_eq ((X-Y) mod wB) (X-Y)); intros Heq.
+ destruct Zcompare; intros;
+  [ rewrite phi_phi_inv; auto | now apply H1 | now apply H1].
+ Qed.
+
+ Lemma spec_sub_carry_c : forall x y, [-|w_sub_carry_c x y|] = [|x|] - [|y|] - 1.
+ Proof.
+ clear; unfold w_sub_carry_c; simpl; intros.
+ unfold sub31carryc, sub31, interp_carry; intros.
+ rewrite phi_phi_inv.
+ generalize (spec_to_Z x)(spec_to_Z y); intros.
+ set (X:=[|x|]) in *; set (Y:=[|y|]) in *; clearbody X Y.
+
+ assert ((X-Y-1) mod wB ?= X-Y-1 <> Eq -> [-|C1 (phi_inv (X-Y-1))|] = X-Y-1).
+  unfold interp_carry; rewrite phi_phi_inv, Zcompare_Eq_iff_eq; intros.
+  destruct (Z_lt_le_dec (X-Y-1) 0).
+  rewrite <- (Z_mod_plus_full (X-Y-1) 1 wB).
+  rewrite Zmod_small; romega.
+  contradict H1; apply Zmod_small; romega.
+
+ generalize (Zcompare_Eq_eq ((X-Y-1) mod wB) (X-Y-1)); intros Heq.
+ destruct Zcompare; intros; 
+  [ rewrite phi_phi_inv; auto | now apply H1 | now apply H1].
+ Qed.
+
+ Lemma spec_sub : forall x y, [|w_sub x y|] = ([|x|] - [|y|]) mod wB.
+ Proof.
+ clear; unfold w_sub; simpl; intros.
+ apply phi_phi_inv.
+ Qed.
+
+ Lemma spec_sub_carry :
+   forall x y, [|w_sub_carry x y|] = ([|x|] - [|y|] - 1) mod wB.
+ Proof.
+ clear; unfold w_sub_carry; simpl; intros.
+ unfold sub31.
+ repeat rewrite phi_phi_inv.
+ apply Zminus_mod_idemp_l.
+ Qed.
+
+ Lemma spec_opp_c : forall x, [-|w_opp_c x|] = -[|x|].
+ Proof. 
+ clear - w_sub_c; unfold w_opp_c; simpl; intros.
+ apply spec_sub_c.
+ Qed.
+
+ Lemma spec_opp : forall x, [|w_opp x|] = (-[|x|]) mod wB.
+ Proof.
+ clear; unfold w_opp; simpl; intros.
+ apply phi_phi_inv.
+ Qed.
+
+ Lemma spec_opp_carry : forall x, [|w_opp_carry x|] = wB - [|x|] - 1.
+ Proof.
+ clear; unfold w_opp_carry, znz_opp_carry, int31_op; intros.
+ unfold sub31.
+ repeat rewrite phi_phi_inv.
+ change [|1|] with 1; change [|0|] with 0.
+ rewrite <- (Z_mod_plus_full (0-[|x|]) 1 wB).
+ rewrite Zminus_mod_idemp_l.
+ rewrite Zmod_small; generalize (spec_to_Z x); romega.
+ Qed.
+
+ Lemma spec_pred_c : forall x, [-|w_pred_c x|] = [|x|] - 1.
+ Proof.
+ clear -w_sub_c; unfold w_pred_c; simpl; intros.
+ apply spec_sub_c.
+ Qed.
+
+ Lemma spec_pred : forall x, [|w_pred x|] = ([|x|] - 1) mod wB.
+ Proof.
+ clear -w_sub; unfold w_pred; simpl; intros.
+ apply spec_sub.
+ Qed.
+
+ (** Multiplication *)
+
+ Let w_mul_c       := int31_op.(znz_mul_c).
+ Let w_mul         := int31_op.(znz_mul).
+ Let w_square_c    := int31_op.(znz_square_c).
+
+ Lemma phi2_phi_inv2 : forall x, [||phi_inv2 x||] = x mod (wB^2).
+ Proof.
+ assert (forall z, (z / wB) mod wB * wB + z mod wB = z mod wB ^ 2).
+  intros.
+  assert ((z/wB) mod wB = z/wB - (z/wB/wB)*wB).
+   rewrite (Z_div_mod_eq (z/wB) wB wB_pos) at 2; ring.
+  assert (z mod wB = z - (z/wB)*wB).
+   rewrite (Z_div_mod_eq z wB wB_pos) at 2; ring.
+  rewrite H.
+  rewrite H0 at 1.
+  ring_simplify.
+  rewrite Zdiv_Zdiv; auto with zarith.
+  rewrite (Z_div_mod_eq z (wB*wB)) at 2; auto with zarith.
+  change (wB*wB) with (wB^2); ring.
+
+ unfold phi_inv2.
+ destruct x; unfold zn2z_to_Z; rewrite ?phi_phi_inv; 
+  change base with wB; auto.
+ Qed.
+
+ Lemma spec_mul_c : forall x y, [|| w_mul_c x y ||] = [|x|] * [|y|].
+ Proof.
+ clear; unfold w_mul_c; simpl; intros.
+ unfold mul31c.
+ rewrite phi2_phi_inv2.
+ apply Zmod_small.
+ generalize (spec_to_Z x)(spec_to_Z y); intros.
+ change (wB^2) with (wB * wB).
+ auto using Zmult_lt_compat with zarith.
+ Qed.
+
+ Lemma spec_mul : forall x y, [|w_mul x y|] = ([|x|] * [|y|]) mod wB.
+ Proof.
+ clear; unfold w_mul; simpl; intros.
+ apply phi_phi_inv.
+ Qed.
+
+ Lemma spec_square_c : forall x, [|| w_square_c x||] = [|x|] * [|x|].
+ Proof.
+ clear -w_mul_c; unfold w_square_c; simpl; intros.
+ apply spec_mul_c.
+ Qed.
+
+ (** Division *) 
+
+ Let w_div21       := int31_op.(znz_div21).
+ Let w_div_gt      := int31_op.(znz_div_gt).
+ Let w_div         := int31_op.(znz_div).
+
+ Let w_mod_gt      := int31_op.(znz_mod_gt).
+ Let w_mod         := int31_op.(znz_mod).
+ Let w_gcd_gt      := int31_op.(znz_gcd_gt).
+ Let w_gcd         := int31_op.(znz_gcd).
+
+ Let w_add_mul_div := int31_op.(znz_add_mul_div).
+
+ Let w_pos_mod     := int31_op.(znz_pos_mod).
+
+ Lemma spec_div21 : forall a1 a2 b,
+      wB/2 <= [|b|] ->
+      [|a1|] < [|b|] ->
+      let (q,r) := w_div21 a1 a2 b in
+      [|a1|] *wB+ [|a2|] = [|q|] * [|b|] + [|r|] /\
+      0 <= [|r|] < [|b|].
+ Proof.
+ unfold w_div21, znz_div21; simpl; unfold div3121.
+ intros.
+ generalize (spec_to_Z a1)(spec_to_Z a2)(spec_to_Z b); intros.
+ assert ([|b|]>0) by (auto with zarith).
+ generalize (Z_div_mod (phi2 a1 a2) [|b|] H4) (Z_div_pos (phi2 a1 a2) [|b|] H4).
+ unfold Zdiv; destruct (Zdiv_eucl (phi2 a1 a2) [|b|]); simpl.
+ rewrite ?phi_phi_inv.
+ destruct 1; intros.
+ unfold phi2 in *.
+ change base with wB; change base with wB in H5.
+ change (Zpower_pos 2 31) with wB; change (Zpower_pos 2 31) with wB in H.
+ rewrite H5, Zmult_comm.
+ replace (z0 mod wB) with z0 by (symmetry; apply Zmod_small; omega).
+ replace (z mod wB) with z; auto with zarith.
+  symmetry; apply Zmod_small.
+  split.
+  apply H7; change base with wB; auto with zarith.
+  apply Zmult_gt_0_lt_reg_r with [|b|].
+  omega.
+  rewrite Zmult_comm.
+  apply Zle_lt_trans with ([|b|]*z+z0).
+  omega.
+  rewrite <- H5.
+  apply Zle_lt_trans with ([|a1|]*wB+(wB-1)).
+  omega.
+  replace ([|a1|]*wB+(wB-1)) with (wB*([|a1|]+1)-1) by ring.
+  assert (wB*([|a1|]+1) <= wB*[|b|]); try omega.
+  apply Zmult_le_compat; omega.
+ Qed.
+
+ Lemma spec_div : forall a b, 0 < [|b|] ->
+      let (q,r) := w_div a b in
+      [|a|] = [|q|] * [|b|] + [|r|] /\
+      0 <= [|r|] < [|b|].
+ Proof.
+ intros.
+ unfold w_div, znz_div; simpl; unfold div31.
+ assert ([|b|]>0) by (auto with zarith).
+ generalize (Z_div_mod [|a|] [|b|] H0) (Z_div_pos [|a|] [|b|] H0).
+ unfold Zdiv; destruct (Zdiv_eucl [|a|] [|b|]); simpl.
+ rewrite ?phi_phi_inv.
+ destruct 1; intros.
+ rewrite H1, Zmult_comm.
+ generalize (spec_to_Z a)(spec_to_Z b); intros.
+ replace (z0 mod wB) with z0 by (symmetry; apply Zmod_small; omega).
+ replace (z mod wB) with z; auto with zarith.
+  symmetry; apply Zmod_small.
+  split; auto with zarith.
+  apply Zle_lt_trans with [|a|]; auto with zarith.
+  rewrite H1.
+  apply Zle_trans with ([|b|]*z); try omega.
+  rewrite <- (Zmult_1_l z) at 1.
+  apply Zmult_le_compat; auto with zarith.
+ Qed.
+ Lemma spec_div_gt : forall a b, [|a|] > [|b|] -> 0 < [|b|] ->
+      let (q,r) := w_div_gt a b in
+      [|a|] = [|q|] * [|b|] + [|r|] /\
+      0 <= [|r|] < [|b|].
+ Proof.
+ intros; apply spec_div; auto.
+ Qed.
+
+ Lemma spec_mod :  forall a b, 0 < [|b|] ->
+      [|w_mod a b|] = [|a|] mod [|b|].
+ Proof.
+ intros.
+ unfold w_mod, znz_mod; simpl; unfold div31.
+ assert ([|b|]>0) by (auto with zarith).
+ unfold Zmod.
+ generalize (Z_div_mod [|a|] [|b|] H0).
+ destruct (Zdiv_eucl [|a|] [|b|]); simpl.
+ rewrite ?phi_phi_inv.
+ destruct 1; intros.
+ generalize (spec_to_Z b); intros.
+ apply Zmod_small; omega.
+ Qed.
+ Lemma spec_mod_gt : forall a b, [|a|] > [|b|] -> 0 < [|b|] ->
+      [|w_mod_gt a b|] = [|a|] mod [|b|].
+ Proof.
+ intros; apply spec_mod; auto.
+ Qed.
+
+ Lemma spec_gcd : forall a b, Zis_gcd [|a|] [|b|] [|w_gcd a b|].
+ Proof.
+ Admitted. (* TODO !! *)
+ Opaque gcd31.
+ Lemma spec_gcd_gt : forall a b, [|a|] > [|b|] ->
+      Zis_gcd [|a|] [|b|] [|w_gcd_gt a b|].
+ Proof. 
+ intros; apply spec_gcd; auto.
+ Qed.
+
+ Lemma spec_add_mul_div : forall x y p,
+       [|p|] <= Zpos 31 ->
+       [| w_add_mul_div p x y |] =
+         ([|x|] * (2 ^ [|p|]) +
+          [|y|] / (2 ^ ((Zpos 31) - [|p|]))) mod wB.
+ Admitted. (* TODO !! *)
+ Lemma spec_pos_mod : forall w p,
+       [|w_pos_mod p w|] = [|w|] mod (2 ^ [|p|]).
+ Admitted. (* TODO !! *)
+
+ (** Shift operations *)
+
+ Let w_head0       := int31_op.(znz_head0).
+ Let w_tail0       := int31_op.(znz_tail0).
+ 
+
+ Lemma spec_head00:  forall x, [|x|] = 0 -> [|w_head0 x|] = Zpos 31.
+ Proof.
+  intros.
+  generalize (phi_inv_phi x).
+  rewrite H; simpl.
+  intros H'; rewrite <- H'.
+  simpl; auto.
+ Qed.
+ Lemma spec_head0  : forall x,  0 < [|x|] ->
+	 wB/ 2 <= 2 ^ ([|w_head0 x|]) * [|x|] < wB.
+ Admitted. (* TODO !! *)
+ Lemma spec_tail00:  forall x, [|x|] = 0 -> [|w_tail0 x|] = Zpos 31.
+ Proof.
+  intros.
+  generalize (phi_inv_phi x).
+  rewrite H; simpl.
+  intros H'; rewrite <- H'.
+  simpl; auto.
+ Qed.
+ Lemma spec_tail0  : forall x, 0 < [|x|] -> 
+         exists y, 0 <= y /\ [|x|] = (2 * y + 1) * (2 ^ [|w_tail0 x|]).
+ Admitted. (* TODO !! *)
+    
+ (* Sqrt *)
+
+ Let w_sqrt2       := int31_op.(znz_sqrt2).
+ Let w_sqrt        := int31_op.(znz_sqrt).
+
+ Lemma spec_sqrt2 : forall x y,
+       wB/ 4 <= [|x|] ->
+       let (s,r) := w_sqrt2 x y in
+          [||WW x y||] = [|s|] ^ 2 + [+|r|] /\
+          [+|r|] <= 2 * [|s|].
+ Admitted. (* TODO !! *)
+ Lemma spec_sqrt : forall x,
+       [|w_sqrt x|] ^ 2 <= [|x|] < ([|w_sqrt x|] + 1) ^ 2.
+ Admitted. (* TODO !! *)
+  
+ (* Even *)
+ 
+ Let w_is_even     := int31_op.(znz_is_even).
+
+ Lemma spec_is_even : forall x,
+      if w_is_even x then [|x|] mod 2 = 0 else [|x|] mod 2 = 1.
+ Proof.
+ clear; unfold w_is_even; simpl; intros.
+ Admitted. (* TODO !! *)
+
+ (* The following definition is verrry slooow  
+    without the two Opaque  (??) *)
+ Opaque gcd31.
+ Opaque addmuldiv31.
+
+ Definition int31_spec : znz_spec int31_op.
+  split.
+  exact    spec_to_Z.
+  exact    positive_to_int31_spec.
+  exact    spec_zdigits.
+  exact    spec_more_than_1_digit.
+
+  exact    spec_0.
+  exact    spec_1.  
+  exact    spec_Bm1.
+  exact    spec_WW.
+  exact    spec_0W. 
+  exact    spec_W0.
+
+  exact    spec_compare.
+  exact    spec_eq0.
+
+  exact    spec_opp_c. 
+  exact    spec_opp.
+  exact    spec_opp_carry.
+
+  exact    spec_succ_c.
+  exact    spec_add_c.
+  exact    spec_add_carry_c.
+  exact    spec_succ.
+  exact    spec_add.
+  exact    spec_add_carry.
+
+  exact    spec_pred_c.
+  exact    spec_sub_c.
+  exact    spec_sub_carry_c.
+  exact    spec_pred.
+  exact    spec_sub.
+  exact    spec_sub_carry.
+
+  exact    spec_mul_c.
+  exact    spec_mul.
+  exact    spec_square_c.
+
+  exact    spec_div21.
+  exact    spec_div_gt. 
+  exact    spec_div.
+
+  exact    spec_mod_gt.
+  exact    spec_mod.
+
+  exact    spec_gcd_gt.
+  exact    spec_gcd.
+
+  exact    spec_head00.
+  exact    spec_head0.
+  exact    spec_tail00. 
+  exact    spec_tail0.
+
+  exact    spec_add_mul_div.
+  exact    spec_pos_mod.
+
+  exact    spec_is_even.
+  exact    spec_sqrt2.
+  exact    spec_sqrt.
+ Qed.
+
+ Transparent gcd31.
+ Transparent addmuldiv31.
+
+End Int31_Spec.
 
 
 Module Int31Cyclic <: CyclicType.
